Try to abstract STLC, but going to revert

src/Eval.v
@@ -4,7 +4,8 @@ Require Import
   Ty
   Exp
   Sub
-  Sem.
+  Sem
+  Lang.
 
 From Equations Require Import Equations.
 Set Equations With UIP.
@@ -16,34 +17,41 @@ Import ListNotations.
 Section Eval.
 
 Context {t : Type}.
-Context {x : Ty t → Type}.
-Context `{Sem t x}.
+Context {x : Env t → Ty t → Type}.
+Context `{Lang t x}.
 
 Inductive Eval : ∀ {τ}, Exp t x [] τ → Exp t x [] τ → Prop :=
-  | EvAbs t1 t2 (e : Exp t x [t1] t2) :
+  | EvTerm t1 (e1 : x [] t1) (e2 : Exp t x [] t1) :
+    eval e1 e2 →
+    Eval (TERM e1) e2
+
+  | EvLam t1 t2 (e : Exp t x [t1] t2) :
     Eval (LAM e) (LAM e)
 
   | EvApp t1 t2 e v w (e1 : Exp t x [] (t1 ⟶ t2)) e2 :
-    Eval e1 (LAM e) → Eval e2 w → Eval (STmExp {| w |} e) v →
+    Eval e1 (LAM e) →
+    Eval e2 w →
+    Eval (STmExp (ren:=@ren _ _ _) (sub:=@sub _ _ _) {| w |} e) v →
     Eval (APP e1 e2) v.
 
-Theorem Soundness τ (e : Exp t x [] τ) v :
-  Eval e v → SemExp SemT SemX e = SemExp SemT SemX v.
+Theorem soundness τ (e : Exp t x [] τ) v :
+  Eval e v → SemExp SemT (@SemX _ _ _) e = SemExp SemT (@SemX _ _ _) v.
 Proof.
   intros.
   induction H0; simpl; auto.
-  extensionality E.
-  destruct E.
-  rewrite IHEval1.
-  rewrite IHEval2.
-  rewrite <- IHEval3.
-  simpl.
-  rewrite <- SemSubComm.
-  - simpl.
-    unfold hdSub.
-    now rewrite consSub_equation_1.
-  - now apply SemX_SemRen.
-  - now apply SemX_SemSub.
+  - now apply (eval_sound _ e1 e2).
+  - extensionality E.
+    destruct E.
+    rewrite IHEval1.
+    rewrite IHEval2.
+    rewrite <- IHEval3.
+    simpl.
+    rewrite <- SemSubComm.
+    + simpl.
+      unfold hdSub.
+      now rewrite consSub_equation_1.
+    + now intros; apply SemX_SemRen.
+    + now intros; apply SemX_SemSub.
 Qed.
 
 End Eval.
