src/Pact.v
@@ -3,8 +3,10 @@ Require Import
   Coq.Lists.List
   Ty
   Exp
+  Ren
   Sub
-  Sem.
+  Sem
+  Lang.
 
 From Equations Require Import Equations.
 Set Equations With UIP.
@@ -15,14 +17,52 @@ Import ListNotations.
 
 Section Pact.
 
+(** Pact syntax *)
+
 Inductive PactTy : Type :=
   | TUnit : PactTy
   | TList : Ty PactTy → PactTy.
 
-Inductive PactExpr : Ty PactTy → Type :=
-  | Unit : PactExpr (TYP TUnit)
-  | Nil {τ} : PactExpr (TYP (TList τ))
-  | Cons {τ} : PactExpr τ → PactExpr (TYP (TList τ)) → PactExpr (TYP (TList τ)).
+Inductive PactExpr Γ : Ty PactTy → Type :=
+  | Unit : PactExpr Γ (TYP TUnit)
+  | Nil {τ} : PactExpr Γ (TYP (TList τ))
+  | Cons {τ} : Exp PactTy PactExpr Γ τ →
+               Exp PactTy PactExpr Γ (TYP (TList τ)) →
+               PactExpr Γ (TYP (TList τ)).
+
+Arguments Unit {Γ}.
+Arguments Nil {Γ τ}.
+Arguments Cons {Γ τ} _ _.
+
+Fixpoint PactRen {Γ Γ' τ} (r : Ren Γ Γ') (p : PactExpr Γ τ) : PactExpr Γ' τ :=
+  match p with
+  | Unit => Unit
+  | Nil => Nil
+  | @Cons _ τ x xs =>
+    Cons (@RTmExp _ _ (@PactRen) Γ Γ' _ r x)
+         (RTmExp (ren:=@PactRen) r xs)
+  end.
+
+Fixpoint PactSub {Γ Γ' τ} (r : Sub Γ Γ') (p : PactExpr Γ τ) : PactExpr Γ' τ :=
+  match p with
+  | Unit => Unit
+  | Nil => Nil
+  | @Cons _ τ x xs =>
+    Cons (@STmExp _ _ (@PactRen) (@PactSub) Γ Γ' _ r x)
+         (STmExp (ren:=@PactRen) (sub:=@PactSub) r xs)
+  end.
+
+(** Pact evaluation *)
+
+Inductive PactEval : ∀ {τ}, PactExpr [] τ → Exp PactTy PactExpr [] τ → Prop :=
+  | EvUnit : PactEval (@Unit []) (TERM (@Unit []))
+  | EvNil {τ} : PactEval (@Nil _ τ) (TERM (@Nil _ τ))
+  | EvCons {τ} (x : PactExpr [] τ) x' (xs : PactExpr [] (TYP (TList τ))) xs' :
+    PactEval x x' →
+    PactEval xs xs' →
+    PactEval (Cons (TERM x) (TERM xs)) (TERM (Cons x' xs')).
+
+(** Pact semantics *)
 
 Fixpoint SemPactTy (t : PactTy) : Type :=
   match t with
@@ -30,26 +70,35 @@ Fixpoint SemPactTy (t : PactTy) : Type :=
   | TList y => list (SemTy SemPactTy y)
   end.
 
-Fixpoint SemPactExpr {Γ τ} (r : PactExpr τ)
+Fixpoint SemPactExpr {Γ τ} (r : PactExpr Γ τ)
          (E : SemEnv SemPactTy Γ) : SemTy SemPactTy τ :=
   match r with
   | Unit => tt
   | Nil => []
-  | Cons x xs => SemPactExpr x E :: SemPactExpr xs E
+  | Cons x xs =>
+    SemExp SemPactTy (@SemPactExpr) x E :: SemExp SemPactTy (@SemPactExpr) xs E
   end.
 
 #[export]
-Program Instance Pact_Sem : Sem PactTy PactExpr := {
+Program Instance Pact_Lang : Lang PactTy PactExpr := {
+  ren  := @PactRen;
+  sub  := @PactSub;
+  eval := @PactEval;
   SemT := SemPactTy;
-  SemX := @SemPactExpr
+  SemX := @SemPactExpr;
 }.
 Next Obligation.
   induction z; simpl; auto.
-  now rewrite IHz1, IHz2.
+  now rewrite !H.
 Qed.
 Next Obligation.
   induction z; simpl; auto.
-  now rewrite IHz1, IHz2.
+  now rewrite !H.
+Qed.
+Next Obligation.
+  induction H; simpl; auto.
+  extensionality E.
+  now rewrite IHPactEval1, IHPactEval2.
 Qed.
 
 End Pact.
